theories/Labelled_Transition_System/Definitions/gLts.v
@@ -44,12 +44,13 @@ Class ExtAction (A : Type) :=
       non_blocking η → dual η ɣ → 
         ¬ non_blocking ɣ ;
 
-      (* Unique non-blocking action *)
-      co : A → A;
-      unique_nb η ɣ: non_blocking η → dual η ɣ → η = (co ɣ);
+      (* Without dual, an action isn't observable *)
+      exists_duo_nb μ : { η | dual η μ };
 
-      (* Handy hypothesis *)
-      exists_duo_nb η : exists μ, dual η μ;
+      (* Unique non-blocking action *)
+      unique_nb η ɣ: non_blocking η → dual η ɣ → η = proj1_sig (exists_duo_nb ɣ);
+
+      (* Handy Hypothesis *)
       nb_not_nb η1 η2 ɣ : non_blocking η1 → dual η1 ɣ → dual η2 ɣ → non_blocking η2;
       duo_sym : Symmetric dual;
       (* Can we derive these hypothesis ?*)
@@ -93,16 +94,11 @@ intros. destruct (decide (non_blocking μ)) as [nb | not_nb].
   + right. intro Hyp. destruct Hyp as (μ' & nb' & duo').
     assert (blocking μ).
     eapply dual_blocks; eauto. contradiction.
-  + destruct (decide (non_blocking (co μ))) as [nb' | not_nb'].
-    ++ assert { μ' | dual μ μ'} as (μ' & duo).
-       exact (choice (fun μ0 => dual μ μ0) (exists_duo_nb μ) ).
-       symmetry in duo.
-       destruct (decide (non_blocking μ')) as [nb'' | not_nb''].
-       +++ left. exists μ'; eauto.
-       +++ right. intro Hyp. destruct Hyp as (μ'' & nb'' & duo'').
-           assert (non_blocking μ'). eapply nb_not_nb; eauto. contradiction.
+  + destruct (decide (non_blocking (proj1_sig (exists_duo_nb μ)))) as [nb' | not_nb'].
+    ++ left. exists (proj1_sig (exists_duo_nb μ)) ; eauto.
+       split. eauto. exact (proj2_sig (exists_duo_nb μ)).
     ++ right. intro imp. destruct imp as (η'' & nb'' & duo).
-       assert (η'' = (co μ)). eapply unique_nb; eauto. subst.
+       assert (η'' = (proj1_sig (exists_duo_nb μ))). eapply unique_nb; eauto. subst.
        contradiction.
 Qed.
 
